Finish `u256.from_bytes`
This is now working, though I have gotten very stuck trying to show
simple examples of it.  That's concerning since it means I probably
cannot show many useful properties!

src/LeanEVM/Byte.lean
@@ -6,36 +6,31 @@ opaque BYTE_0 : byte := {val:=0, isLt:=(by simp)}
 
 -- Construct a natural number from a sequence of one or more bytes store in big
 -- endian form.
-def from_bytes_be(bytes:Array byte)(i: Fin bytes.size) : Nat := 
+def from_bytes_be(bytes:List byte)(i: Fin bytes.length) : Nat := 
   -- Read ith byte
   let b : byte := bytes[i];
   -- Decide what to do
   if r:i.val = 0 then b.val
   else
     -- Construct i-1
-    let im1 : Fin bytes.size := {val:=i.val-1,isLt:=(
+    let im1 : Fin bytes.length := {val:=i.val-1,isLt:=(
       by 
         have p : i.val-1 < i.val := (Nat.pred_lt r);
         linarith [i.isLt])
     };
     -- Done
     (256 * (from_bytes_be bytes im1)) + b.val
-  termination_by
-    from_bytes_be _ i => (i.val)  
-
-example (n:Nat): [n][0] = n := 
-by
-  simp
 
 -- Prove that converting an array consisting of a single byte generates the
 -- corresponding Nat.
-example (i:Fin 1)(b:byte): (from_bytes_be #[b] i) = b.val :=
+example (n:byte)(i:Fin 1): (from_bytes_be [n] i) = n.val :=
 by 
-  have p:i=0 := by simp;
+  let arr := [n];
   unfold from_bytes_be
-  --simp_arith
-  simp [*]
-  unfold Fin.val
+  have p:i={val:=0,isLt:=(by simp)} := (by simp);  
+  have q:i=0 := by sorry;
+  have z:arr[0]=n := by sorry;
+  rw [q]
+  rw [<-z]
+  simp_all
   sorry  
-  
-  
